# MTH 180 Concepts

````````` {div} full-width
``````` {dropdown} <iframe width="100%" height="600" src="https://www.youtube.com/embed/UgUcN0c0ZSw" title="YouTube video player" frameborder="0" allow="accelerometer; autoplay; clipboard-write; encrypted-media; gyroscope; picture-in-picture; web-share" allowfullscreen></iframe>

**Additional Resources**

``` {card} Disclaimer
The following sets of videos have been vetted for the general knowledge of mathematical subject matter applicable to CSC 212 but not directly focused on. This is not an exhaustive list, but a guide to helpful instruction. The variety in selection is merely to help fit the multitude of learning curves for students within the course.
```
``` {card} Pre-calculas w/ Professor Leonard

- [Introduction to Sequences](https://youtu.be/c5D7BJ-R41I) : 53:35
- [Introduction to Series and Summation Notation](https://youtu.be/Ipz9xXeoaRc) : 42:41
- [Arithmetic Sequences](https://youtu.be/bxGmjouB6t4) : 21:31
- [Arithmetic Series](https://youtu.be/XdXQjHsl4q0) : 15:11
- [Geometric Sequences](https://youtu.be/qyHCnYewdrQ) : 30:14
- [Geometric Series](https://youtu.be/_yDqkrbd5mk) : 42:02
- [Proof by Mathematical Induction](https://youtu.be/x5cWX-EyLEI) : 22:35
```
``` {card} The Organic Chemistry Tutor
- [Arithmetic Sequences and Arithmetic Series - Basic Introduction](https://youtu.be/XZJdyPkCxuE) : 44:03
- [Geometric Series and Geometric Sequences - Basic Introduction](https://youtu.be/zRKZ0-kOUZM) : 31:19
- [Finding The Sum of a Finite Geometric Series](https://youtu.be/uAnJmAFBpak) : 12:58
- [Finding The Sum of an Infinite Geometric Series](https://youtu.be/jxRqRLMliPc) : 19:49
- [Telescoping Series](https://youtu.be/XVkdhU6nJbo) : 23:38
```
``` {card} Prof D
- [Sequence and Series | Terms of Sequence and Associated Series | Pre-Calculus](https://youtu.be/ZcqCgF_3_yo) : 11:46
- [Properties of Sigma Notation and Summation Formulas | Pre-Calculus](https://youtu.be/-CvVstoSwd4) : 11:18
- [Evaluating Sigma Notation | Summation Formulas | Pre-Calculus](https://youtu.be/S0hqm5r-1jQ) : 7:47
- [Writing Summations in Sigma Notation | Series and Sigma Notation | Pre-Calculus](https://youtu.be/app1HDQ_u4k) : 10:37
- [Proof by Mathematical Induction | Principle of Mathematical Induction | Sample Problems | Part 1](https://youtu.be/cF-SqFM56Qc) : 13:23
- [Proof by Mathematical Induction | Pre-Calculus](https://youtu.be/dYC_y6kuUuc) : 12:54
- [Proof by Mathematical Induction | Part 3 | Pre-Calculus](https://youtu.be/ei_6MmUdEWY) : 12:37
- [Proof by Mathematical Induction | Part 4 | Pre-Calculus](https://youtu.be/OUTAFY5dLNg) : 8:00
```
``` {card} TrevTutor & Kimberly Brehm
- [RECURRENCE RELATIONS - DISCRETE MATHEMATICS](https://youtu.be/eAaP4XaB8hM) : 15:24
- [Discrete Math - 2.4.2 Recurrence Relations](https://youtu.be/QaAQ-bKCUME) : 15:06
- [Discrete Math - 8.1.1 Modeling with Recurrence Relations | Kimberly Brehm](https://youtu.be/awR_p6J7Lyg) : 25:27
```

```````
`````````

## Sequences

``````````` {div} full-width
`````````` {card}

``` {glossary}
Sequence
  a function whose domain is the set of *positive* integers  
  ex: $\{ 1, 2, 3, 4, \dots \}$
```

The general, or $n^{th}$ term, is denoted as $a_n$

``` {list-table}
* - $odd\ integers$
  - $1$
  - $3$
  - $5$
  - $7$
  - $9$
  - $\dots$
  - $n$
* - $perfect\ squares$
  - $1$
  - $4$
  - $9$
  - $16$
  - $25$
  - $\dots$
  - $n$
* - 
  - $a_1$
  - $a_2$
  - $a_3$
  - $a_4$
  - $a_5$
  - $\dots$
  - $a_n$
```

``````` {admonition} Try it 
:class: hint
Write out the first five (5) terms of the sequence...

`````` {dropdown} $a_n = 2n + 3$

$$\begin{align}  
a_1 & = 2(1) + 3 & = 5 \\
a_2 & = 2(2) + 3 & = 7 \\
a_3 & = 2(3) + 3 & = 9 \\
a_4 & = 2(4) + 3 & = 11 \\
a_5 & = 2(5) + 3 & = 13 \\
\end{align}$$

$$first\ five\ (5)\ terms\ of\ the\ sequence\ $$
$$ \{ 5, 7, 9, 11, 13 \} $$
``````

`````` {dropdown} $a_n = (-1)^n * \frac{6 - 2n}{ \sqrt{n + 1}} $
`````  {tab-set}
````   {tab-item} a_1
$$\begin{align}  
a_1 & = (-1)^{1} * \frac{6 - 2(1)}{ \sqrt{(1) + 1}} \\
& = \frac{-4}{\sqrt{-2}} \\
& = \frac{-4 \sqrt{-2}}{2} \\
& = -2 \sqrt{-2} \\
\end{align}$$
````
````   {tab-item} a_2
$$\begin{align}  
a_2 & = (-1)^{2} * \frac{6 - 2(2)}{ \sqrt{(2) + 1}} \\
& = \frac{2}{\sqrt{3}} \\
& = \frac{2 \sqrt{3}}{3} \\
\end{align}$$
````
````   {tab-item} a_3
$$\begin{align}  
a_3 & = (-1)^{3} * \frac{6 - 2(3)}{ \sqrt{(3) + 1}} \\
& = \frac{-0}{\sqrt{4}} \\
& = 0 \\
\end{align}$$
````
````   {tab-item} a_4
$$\begin{align}  
a_4 & = (-1)^{4} * \frac{6 - 2(4)}{ \sqrt{(4) + 1}} \\
& = \frac{-2}{\sqrt{5}} \\
& = \frac{-2 \sqrt{5}}{5} \\
\end{align}$$
````
````   {tab-item} a_5
$$\begin{align}  
a_5 & = (-1)^{5} * \frac{6 - 2(5)}{ \sqrt{(5) + 1}} \\
& = - \frac{-4}{\sqrt{6}} \\
& = \frac{2 \sqrt{6}}{3} \\
\end{align}$$
````
````   {tab-item} first five
$$first\ five\ (5)\ terms\ of\ the\ sequence\ $$
$$ \{ -2 \sqrt{-2}, \frac{2 \sqrt{3}}{3}, 0, \frac{-2 \sqrt{5}}{5}, \frac{2 \sqrt{6}}{3} \} $$
````
`````
``````
```````

``````` {admonition} Try it 
:class: hint

Write the $n^{th}$ term of the sequence $\{a_n\}$ suggested by the pattern

``` {dropdown} $\frac{2}{3}, \frac{4}{9}, \frac{8}{27}, \frac{16}{81}, \dots $
Find the pattern...

$\frac{2^1}{3^1}, \frac{2^2}{3^2}, \frac{2^3}{3^3}, \frac{2^4}{3^4} $

Therefore,

$$\begin{align}
a_n & = \frac{2^n}{3^n} \\
& = \bigg( \frac{2}{3} \bigg) ^n \\
\end{align}$$
```

```` {dropdown} $ 2, -4, 6, -8, 10, \dots $
Find the pattern...

``` {list-table}

* - $2$
  - $-4$
  - $6$
  - $-8$
  - $10$
  - $\dots$
  - $n$
* - $a_1$
  - $a_2$
  - $a_3$
  - $a_4$
  - $a_5$
  - $\dots$
  - $a_n$
```

``` {card} Check : $a_n = (-1)^n * 2n$
$$\begin{align}
a_1 & = (-1)^1 * 2(1) \\
& = \bbox[5px,border:2px solid red]{ \cancel{-2} }
\end{align}$$
```

``` {card} Check : $a_n = (-1)^{n+1} * 2n$
$$\begin{align}
a_1 & = (-1)^{n+1} * 2(1) \\
& = -1^2 * 2 \\
& = \bbox[5px,border:2px solid green]{ 2 }
\end{align}$$
```

Therefore,

$$\begin{align}
a_n = (-1)^{n+1} * 2n \\
\end{align}$$
````
```````

``` {glossary}
Recursive relation
  a sequence for which the given is the first term together with a rule for obtaining any $a_{n+1}$ from the preceding term $a_n$ for $n \ge 1$
```

``````` {admonition} Try it 
:class: hint

Find the first five (5) terms of the recursively defined infinite sequence

`````` {dropdown} $a_1 = 2, \ \ \ \ \ a_{n+1} = - \frac{n}{a_n}$

````` {grid}
````  {grid-item-card}
:columns: 12

$$\begin{align}
a_1 & = 2 \\
\end{align}$$
````
````  {grid-item-card}
:columns: 6

$$a_2$$

---

$$\begin{align}
a_{n+1} & = a_2 \\
a_2 & = \frac{-1}{a_1} \\
& = \frac{-1}{2} \\
a_{n+1} & = a_3 \\
\end{align}$$
````
````  {grid-item-card}
:columns: 6

$$a_3$$

---

$$\begin{align}
a_3 & = \frac{-2}{a_2} \\
& = \frac{-2}{\frac{-1}{2}} \\
& = 4 \\
\end{align}$$
````
````  {grid-item-card}
:columns: 6

$$a_4$$

---

$$\begin{align}
a_4 & = \frac{-3}{a_3} \\
& = \frac{-3}{4} \\
\end{align}$$
````
````  {grid-item-card}
:columns: 6

$$a_5$$

---

$$\begin{align}
a_5 & = \frac{-4}{a_4} \\
& = \frac{-4}{(\frac{-3}{4})} \\
& = \frac{16}{3} \\
\end{align}$$
````
````  {grid-item-card}
:columns: 12

$$first\ five\ recursive\ terms$$

---

$$\begin{align}
\frac{-1}{2}, 4, \frac{-3}{4}, \frac{16}{3} \ \ \ \ \ \\
\end{align}$$
````
`````
``````

`````` {dropdown} $a_1 = -1, \ \ \ \ \ a_2 = 1, \ \ \ \ \ a_n = a_{n+1} + na_{n-1}$

````` {grid}
````  {grid-item-card}
:columns: 12

$$\begin{align}
a_1 & = -1 \\
a_2 & = 1 \\
\end{align}$$
````
````  {grid-item-card}
:columns: 4

$$a_3$$

---

$$\begin{align}
a_3 & = a_{3-2} + (3 * a_{3-1}) \\
& = a_1 + (3 * a_2) \\
& = -1 + 3(1) \\
& = 2 \\
\end{align}$$
````
````  {grid-item-card}
:columns: 4

$$a_4$$

---

$$\begin{align}
a_4 & = a_{4-2} + (4 * a_{4-1}) \\
& = a_2 + (4 * a_3) \\
& = 1 + 4(1) \\
& = 9 \\
\end{align}$$
````
````  {grid-item-card}
:columns: 4

$$a_3$$

---

$$\begin{align}
a_5 & = a_{5-2} + (5 * a_{5-1}) \\
& = a_3 + (5 * a_4) \\
& = 2 + 5(9) \\
& = 47 \\
\end{align}$$
````
````  {grid-item-card}
:columns: 12

$$first\ five\ recursive\ terms$$

---

$$\begin{align}
-1, 1, 4, 9, 47 \\
\end{align}$$
````
`````
``````
```````
``````````
```````````

## Series

``````````` {div} full-width
`````````` {card}

``` {glossary}
Series
  the *sum* of a number of terms in a sequence
```

```` {grid}
``` {grid-item-card}

$$ can\ be\ finite $$

---

$$ 1 + 3 + 5 + 7 $$
```
``` {grid-item-card}

$$ can\ be\ infinite $$

---

$$ 1 + 3 + 5 + 7 + \bbox[5px,border:2px solid green]{ \dots } $$
$$ 1 + \frac{1}{2} + \frac{1}{4} + \frac{1}{8} + \bbox[5px,border:2px solid green]{ \dots } $$
```
````

````` {card} Summation / Sigma Notation

``` {figure} https://knowledgeuniverseonline.com/wp-content/uploads/2022/03/sigma-notation.png
```

````  {grid}
```   {grid-item-card}
:columns: 4

$$ k-index\ of \\ summation $$

---

$n$ = stopping point  
$ \sum $ = $sigma$ or "sum of"  
$k$ = starting point  
$a_k$ = formula for each term  

```
```   {grid-item-card}
:columns: 8

Example

---

$$ \sum_{k=1}^{n} a_k = a_1 + a_2 + a_3 + a_4 + \dots + a_{n-1} + a_n $$

```
````
`````

````` {admonition} Try it
:class: tip

Write out each sum (expand and simplify)

```` {dropdown} $ \sum_{k=1}^{6} \frac{3}{k+1} $
$$\begin{align}
\sum_{k=1}^{6} \frac{3}{k+1} & = \frac{3}{1+1} + \frac{3}{2+1} + \frac{3}{3+1} + \frac{3}{4+1} + \frac{3}{5+1} + \frac{3}{6+1} \\
& = \frac{3}{2} + 1 + \frac{3}{4} + \frac{3}{5} + \frac{1}{2} + \frac{3}{7} \\
& = \frac{669}{140} \\
\end{align}$$
````
`````

````` {admonition} Try it
:class: tip

Express each sum using summation notation

```` {dropdown} $ 1 + 3 + 5 + 7 + \dots + [2(12)-1] $
$$\begin{align}
& 1 & + & 3 & + & 5 & + & 7 & + & \dots & + & [2(12)-1] \\
& \downarrow & & \downarrow & & \downarrow & & \downarrow & & & & \downarrow \\
& a_1 & + & a_2 & + & a_3 & + & a_4 & + & \dots & + & a_{12} \\
\end{align}$$

``` {card} Check : $a_k = 2k-1$
$$\begin{align}
a_1 & = 2 * 1 - 1 \\
& = \bbox[5px,border:2px solid green]{ 1 } \\
a_2 & = 2 * 2 - 1 \\
& = \bbox[5px,border:2px solid green]{ 3 } \\
a_3 & = 2 * 3 - 1 \\
& = \bbox[5px,border:2px solid green]{ 5 } \\
a_4 & = 2 * 4 - 1 \\
& = \bbox[5px,border:2px solid green]{ 7 } \\
\end{align}$$
```
``` {card} Therefore
$$ \bbox[5px,border:2px solid green]{ \sum_{k=1}^{12} 2k-1 } $$
```
````
`````

````` {admonition} Try it
:class: tip

Find the sum for each sequence

```` {dropdown} $ \sum_{k=1}^{24} -k $
$$\begin{align}
& = (-1) & + & (-2) & + & (-3) & + & (-4) & + & \dots & + & (-24) \\
& = -(1 & + & 2 & + & 3 & + & 4 & + & \dots & + & 24) \\
& = \frac{-24(24+1)}{2} \\
& = -12(25) \\
& = \bbox[5px,border:2px solid green]{ -300 } \\
\end{align}$$

``` {card} 
Formula

$$ \sum_{k=1}^{n} k = 1 + 2 + 3 + \dots + n = \frac{n(n+1)}{2} $$
```

````

```` {dropdown} $ \sum_{k=137}^{428} 2.1 $
$$\begin{align}
& ( 2.1 + 2.1 + \dots + & 2.1 & ) = (2.1)(292) = \bbox[5px,border:2px solid green]{ 613.2 }  \\
& \downarrow & \downarrow \\
& a_{137} & a_{428} &  \\
\\
& \ \ \ 428 \\
& \underline{- 137} \\
& \ \ \ 291 \ iterations
\end{align}$$

``` {card} 
Formula

$$\begin{align} 
\sum_{k=m}^{n} c & = (n - m + 1) c & \\
\sum_{k=137}^{428} 2.1 & = (428 - 137 + 1) 2.1 &  \\
\end{align}$$

---

$c$ = constant
```

````

```` {dropdown} $ \sum_{k=0}^{14} k^2-4 $
$$\begin{align}
& ( 0^2 - 4 ) + ( 1^2 - 4 ) + ( 2^2 - 4 ) + \dots + ( 14^2 - 4 ) = \bbox[5px,border:2px solid green]{ 955 }  \\
\end{align}$$

``` {card} 
Formula

$$\begin{align} 
\sum_{k=1}^{n} (a_k - b_k) & = \sum_{k=1}^{n} a_k - \sum_{k=1}^{n} b_k\\
\\
\\
\sum_{k=0}^{14} (k^2 - 4) & = \sum_{k=0}^{14} k^2 - \sum_{k=0}^{14} 4 \\
\end{align}$$
```

``` {card}
Breakout 1

$$\begin{align} 
\sum_{k=1}^{n} k^2 & = 1^2 + 2^2 + 3^2 + \dots + n^2  & = \frac{n(n+1)(2n+1)}{6} & \\
& & = \frac{14 \bigg(14+1 \bigg) \bigg(2(14)+1 \bigg)}{6} & \\
& & = \bbox[5px,border:2px solid green]{ 1015 } & \\
\end{align}$$
```

``` {card}
Breakout 2

$$\begin{align} 
\sum_{k=1}^{n} 4 & = 4(15) = \bbox[5px,border:2px solid green]{ 60 } \\
\end{align}$$
```

``` {card}
Outcome

$$\begin{align} 
\sum_{k=0}^{14} (k^2 - 4) & = \sum_{k=0}^{14} k^2 - \sum_{k=0}^{14} 4 \\
& = 1015 - 60 \\
& = \bbox[5px,border:2px solid green]{ 955 }
\end{align}$$

````
`````

``````````
```````````